mk_number

binomial_encode.v
@@ -125,3 +125,153 @@ Definition rotate6_270 (l : list bool) :=
 Lemma rotate6_360 l :  rotate6_90 (rotate6_270 l) = l.
 Proof. do 7 (destruct l as [|? l]; simpl; auto). Qed.
 
+(* position x : {0 .. 7} y : {0 ...7}*)
+
+Definition is_valid_pos (xy : nat * nat) := 
+  ((Nat.leb (fst xy) 7) && (Nat.leb (snd xy) 7))%bool.
+
+Definition is_upper_left (xy : nat * nat) :=
+  ((Nat.leb (fst xy) 3) && (Nat.leb (snd xy) 3))%bool.
+
+Definition is_upper_right (xy : nat * nat) :=
+  (negb (Nat.leb (fst xy) 3) && (Nat.leb (snd xy) 3))%bool.
+
+Definition is_lower_left (xy : nat * nat) :=
+  ((Nat.leb (fst xy) 3) && negb (Nat.leb (snd xy) 3))%bool.
+
+Definition is_lower_right (xy : nat * nat) :=
+  (negb (Nat.leb (fst xy) 3) && negb (Nat.leb (snd xy) 3))%bool.
+
+Definition rotatepos_90 (xy : nat * nat) := 
+  (snd xy, 7 - fst xy).
+
+Definition rotatepos_180 (xy : nat * nat) := 
+  rotatepos_90 (rotatepos_90 xy).
+
+Definition rotatepos_270 (xy : nat * nat) := 
+  rotatepos_90 (rotatepos_180 xy).
+
+Lemma rotatepos_360 xy :
+  is_valid_pos xy = true -> rotatepos_90 (rotatepos_270 xy) = xy.
+Proof.
+destruct xy as [x y];
+  do 8 (try destruct x as [|x]);
+  do 8 (try destruct y as [|y]); simpl; auto; try discriminate.
+Qed.
+
+Lemma rotatepos_upper_right xy :
+  is_valid_pos xy = true ->
+  is_upper_right xy = true -> is_upper_left (rotatepos_90 xy) = true.
+Proof.
+destruct xy as [x y];
+  do 8 (try destruct x as [|x]);
+  do 8 (try destruct y as [|y]); simpl; auto; try discriminate.
+Qed.
+
+Lemma rotatepos_lower_right xy :
+  is_valid_pos xy = true ->
+  is_lower_right xy = true -> is_upper_left (rotatepos_180 xy) = true.
+Proof.
+destruct xy as [x y];
+  do 8 (try destruct x as [|x]);
+  do 8 (try destruct y as [|y]); simpl; auto; try discriminate.
+Qed.
+
+Lemma rotatepos_lower_left xy :
+  is_valid_pos xy = true ->
+  is_lower_left xy = true -> is_upper_left (rotatepos_270 xy) = true.
+Proof.
+destruct xy as [x y];
+  do 8 (try destruct x as [|x]);
+  do 8 (try destruct y as [|y]); simpl; auto; try discriminate.
+Qed.
+
+(* direction  0 = Up 1 = Left  2 = Down 3 Rught *)
+
+Definition is_valid_dir (d : nat) := (Nat.leb d 3).
+
+Definition rotatedir_90 d := Nat.modulo (4 + d - 1) 4.
+
+Definition rotatedir_180 (d : nat) := 
+  rotatedir_90 (rotatedir_90 d).
+
+Definition rotatedir_270 (d : nat) := 
+  rotatedir_90 (rotatedir_180 d).
+
+Lemma rotatedir_360 d :
+  is_valid_dir d = true -> rotatedir_90 (rotatedir_270 d) = d.
+Proof.
+do 4 (try destruct d as [|d]); simpl; auto; try discriminate.
+Qed.
+
+Fixpoint lb_to_int (l : list bool) := 
+match l with
+| true :: l1 => (1 + 2 * (lb_to_int l1))%uint63
+| false :: l1 => (2 * (lb_to_int l1))%uint63
+| [] => 0%uint63
+end.
+
+Definition mk_state npos nbin := 
+  let v := lb_to_int (bin_decode 22 6 nbin) in 
+  let cube := (v >> 16)%uint63 in
+  let board := (v land (1 << 16 - 1))%uint63 in 
+  ((cube << 4 + npos) << 16 + board)%uint63.
+
+
+From puzzle Require Import cube.
+Require Import String.
+
+(* Empty board position (0, 0) *)
+Compute print_state (mk_state 0 0).
+(* Empty board position (3, 3) *)
+Compute print_state (mk_state 15 0).
+Compute bin_compute 22 6.
+(* Full board position (0, 0) *)
+Compute print_state (mk_state 0 74613).
+
+(* Function that takes a state and return a direction *)
+Definition get_direction (state : int) : int := 3%uint63.
+
+(* From upper left to full position *)
+Definition ul_to_full (p : int) :=
+  if (p =? 2)%uint63 then 4%uint63 else
+  if (p =? 3)%uint63 then 5%uint63 else p.
+
+(* Function that get the direction from a state *)
+Definition get_dir (s : int) := 3%uint63 (* right *).
+
+From Bignums Require Import BigN.
+Require Import ZArith.
+
+Definition bigN_of_int (z : int) := (BigN.N_of_Z (to_Z z)).
+
+Definition add_state npos nbin (res : bigN) := 
+  let nbit := ((npos + nbin << 2) << 1)%uint63 in
+  let state := mk_state (ul_to_full npos) nbin in 
+  let dir := get_dir state in 
+  (BigN.lor res (BigN.shiftl (bigN_of_int dir) (bigN_of_int nbit)))%bigN.
+
+Definition add_all_pos_state nbin res := 
+let res1 := add_state 0 nbin res in
+let res2 := add_state 1 nbin res1 in
+let res3 := add_state 2 nbin res2 in
+let res4 := add_state 3 nbin res3 in res3.
+
+Fixpoint iter_add_state n nbin res := 
+  let res1 := add_all_pos_state nbin res in 
+  match n with 0 => res1 | S n1 => iter_add_state n1 (nbin + 1) res1 end.
+
+Compute bin_compute 22 6.
+(* 74613 *)
+Definition mk_big_number := iter_add_state 1000 0 0.
+
+Time Compute mk_big_number.
+
+Definition bigN_to_int (z : bigN) := (of_Z (BigN.to_Z z)).
+
+Definition get_dir_from_number npos nbin (num : bigN) := 
+  let nbit := ((npos + nbin << 2) << 1)%uint63 in
+  bigN_to_int (BigN.land (BigN.shiftr num (bigN_of_int nbit)) 3).
+
+Compute get_dir_from_number 0 0 mk_big_number.
+
